heap/basic.lean
@@ -1,0 +1,74 @@
+import data.bitvec
+import data.dlist
+import data.list.perm
+import util.logic
+import util.control.applicative
+import util.control.monad.non_termination
+import util.data.option
+import util.meta.tactic
+
+universes u v w w'
+
+open nat list (hiding bind) function
+
+@[reducible]
+def pointer := ℕ
+
+structure word :=
+to_word :: (to_ptr : ℕ)
+
+instance : has_zero word := ⟨ ⟨ 0 ⟩ ⟩
+instance : has_one word := ⟨ ⟨ 1 ⟩ ⟩
+instance : has_add word := ⟨ λ x y, ⟨ x.to_ptr + y.to_ptr ⟩ ⟩
+
+def heap := pointer → option word
+
+namespace heap
+
+def disjoint (h₀ h₁ : heap) :=
+(∀ p, h₀ p = none ∨ h₁ p = none)
+
+infix ` ## `:51 := disjoint
+
+def part'  (h₀ h₁ : heap) (_ : h₀ ## h₁ . tactic.assumption) : heap
+ | p := h₀ p <|> h₁ p
+
+def maplet (p : pointer) (v : word) : heap
+  | q :=
+if p = q then some v else none
+
+protected def emp : heap :=
+λ _, none
+
+section classical
+
+local attribute [instance] classical.prop_decidable
+
+noncomputable def part  : option heap → option heap → option heap
+| (some hp₀) (some hp₁) :=
+if h : hp₀ ## hp₁
+then some $ part' hp₀ hp₁
+else none
+| _ _ := none
+
+end classical
+
+protected def mk : pointer → list word → heap
+| _ [] := heap.emp
+| p (v :: vs) := λ q, maplet p v q <|> mk (p+1) vs q
+
+protected def delete : pointer → ℕ → heap → heap
+ | p 0 h q := h q
+ | p (succ n) h q :=
+if p = q then none
+else delete (p+1) n h q
+
+protected def insert (hp : heap) (p : pointer) (v : word) : heap
+ | q := if p = q then some v else hp q
+
+def left_combine (h₀ h₁ : heap) : heap
+ | p := h₀ p <|> h₁ p
+
+infix ` <+ `:54 := left_combine
+
+end heap
