heap/default.lean
@@ -1,0 +1,4 @@
+
+import separation.heap.basic
+import separation.heap.lemmas
+import separation.heap.instances
