heap/instances.lean
@@ -1,0 +1,48 @@
+import separation.heap.lemmas
+import util.meta.tactic
+
+universes u
+
+namespace heap
+
+def heap.le (hp₀ hp₁ : heap) : Prop :=
+∃ hp, some hp₁ = part (some hp₀) hp
+
+instance : has_le heap :=
+⟨ heap.le ⟩
+
+instance : partial_order heap :=
+{ le := heap.le
+, le_refl := by { intro x, existsi (some heap.emp), simp, }
+, le_trans := by { introv,
+                   simp [has_le.le,heap.le],
+                   intros hp₀ h₀ hp₁ h₁,
+                   -- have : hp₀ ## hp₁, admit,
+                   existsi part hp₀ hp₁,
+                   simp [h₁,h₀], ac_refl }
+, le_antisymm := by { introv,
+                      simp [has_le.le,heap.le],
+                      intros hp₀ h₀ hp₁ h₁,
+                      simp [h₀,part_assoc] at h₁,
+                      simp [h₁.left] at h₀,
+                      subst b, }
+}
+
+lemma part'_delete_maplet (p : pointer) (v : word) (hp : heap)
+  (h : heap.delete p 1 hp ## maplet p v)
+  (h' : maplet p v ≤ hp)
+: part' (heap.delete p 1 hp) (maplet p v) = hp :=
+begin
+  funext p',
+  by_cases (p = p') with h,
+  { simp [part', heap.delete, maplet, if_pos, h],
+    unfold has_le.le heap.le at h',
+    cases h' with hp' h', cases hp' with hp',
+    { contradiction },
+    have h₂ := eq_part'_of_some_eq_part _ _ _ h',
+    rw [h₂,part',maplet,if_pos h],
+    simp },
+  { simp [part', heap.delete, maplet, if_neg, h] }
+end
+
+end heap
